hw: Add parser for `hw.modty`

Veir/IR/Attribute.lean
@@ -1,6 +1,7 @@
 module
 
 import Veir.ForLean
+public import Std.Data.Iterators.Producers.Array
 
 /-!
   # Attributes
@@ -147,6 +148,38 @@ deriving Inhabited, Repr, DecidableEq, Hashable
 
 end CudaTile
 
+namespace HW
+
+/--
+  The `ModulePort::Direction` type from CIRCT's hw dialect.
+  This represents the direction of a module port.
+-/
+inductive ModulePort.Direction
+| input
+| output
+| inout
+deriving Inhabited, Repr, DecidableEq, Hashable
+
+/--
+  The `ModulePort` type from CIRCT's hw dialect.
+  This represents a port to a module with a direction, type and name.
+-/
+structure ModulePort where
+  name : String
+  type : IntegerType
+  dir : ModulePort.Direction
+deriving Inhabited, Repr, DecidableEq, Hashable
+
+/--
+  The `!hw.modty` type from CIRCT's hw dialect.
+  This represents a list of ports to a module
+-/
+structure ModuleType where
+  ports : Array ModulePort
+deriving Inhabited, Repr, DecidableEq, Hashable
+
+end HW
+
 mutual
 
 /--
@@ -218,6 +251,8 @@ inductive Attribute
 | llvmPointerType (type : LLVM.PointerType)
 /-- Cuda Tile pointer type -/
 | cudaTilePointerType (type : CudaTile.PointerType)
+/-- CIRCT hw module type -/
+| hwModuleType (type : HW.ModuleType)
 deriving Inhabited, Repr, Hashable
 
 end
@@ -363,6 +398,10 @@ def Attribute.decEq (attr1 attr2 : Attribute) : Decidable (attr1 = attr2) := by
     exact (match decEq attr1 attr2 with
       | isTrue hEq => isTrue (by grind)
       | isFalse hEq => isFalse (by grind))
+  case hwModuleType.hwModuleType type1 type2 =>
+    exact (match decEq type1 type2 with
+      | isTrue hEq => isTrue (by grind)
+      | isFalse hEq => isFalse (by grind))
   all_goals exact isFalse (by grind)
 termination_by sizeOf attr1
 end
@@ -434,6 +473,20 @@ instance : ToString LLVM.PointerType where
 instance : ToString CudaTile.PointerType where
   toString ptr := s!"!cuda_tile.ptr<{ptr.pointeeType}>"
 
+instance : ToString HW.ModulePort.Direction where
+  toString
+  | .input => "input"
+  | .output => "output"
+  | .inout => "inout"
+
+instance : ToString HW.ModulePort where
+  toString attr := s!"{attr.dir} {attr.name} : {attr.type}"
+
+instance : ToString HW.ModuleType where
+  toString attr :=
+    let values := attr.ports.iter.map ToString.toString |>.intercalateString ", "
+    s!"!hw.modty<{values}>"
+
 mutual
 
 def ArrayAttr.toString (attr : ArrayAttr) : String :=
@@ -504,6 +557,7 @@ def Attribute.toString (attr : Attribute) : String :=
   | .modArithType type => ToString.toString type
   | .llvmPointerType type => ToString.toString type
   | .cudaTilePointerType type => ToString.toString type
+  | .hwModuleType type => ToString.toString type
 termination_by sizeOf attr
 
 end
@@ -567,6 +621,9 @@ instance : Coe LLVM.PointerType Attribute where
 instance : Coe CudaTile.PointerType Attribute where
   coe type := .cudaTilePointerType type
 
+instance : Coe HW.ModuleType Attribute where
+  coe type := .hwModuleType type
+
 /-!
   ## TypeAttr definition
 
@@ -598,6 +655,7 @@ def isType (attr : Attribute) : Bool :=
   | .registerAttr _ => true
   | .llvmPointerType _ => true
   | .cudaTilePointerType _ => true
+  | .hwModuleType _ => true
 
 @[simp, grind =]
 theorem isType_integerType type : (integerType type).isType = true := by rfl
@@ -612,6 +670,8 @@ theorem isType_modArithType type : (modArithType type).isType = true := by rfl
 theorem isType_llvmPointerType type : (llvmPointerType type).isType = true := by rfl
 @[simp, grind =]
 theorem isType_cudaTilePointerType type : (cudaTilePointerType type).isType = true := by rfl
+@[simp, grind =]
+theorem isType_hwModuleType type : (hwModuleType type).isType = true := by rfl
 
 end Attribute
 
@@ -661,6 +721,9 @@ instance : Coe LLVM.PointerType TypeAttr where
 
 instance : Coe CudaTile.PointerType TypeAttr where
   coe type := ⟨.cudaTilePointerType type, by rfl⟩
+
+instance : Coe HW.ModuleType TypeAttr where
+  coe type := ⟨.hwModuleType type, by rfl⟩
 
 end
 end Veir
